\documentclass[../CryptoHW3.tex]{subfiles}

\begin{document}
\begin{flushleft}



\numbpr{7}
\prob{7}  We start with $a^{\phi \left( N \right)} = 1 \mod N$ and note $\phi \left( N \right) = \phi \left( p \right) \, \phi \left( q \right)$ to obtain

\begin{align}
  a^{\phi \left( N \right)} = 1 \mod N = a^{\phi \left( p \right) \, \phi \left( q \right)} \notag
\end{align}
  
Since $\phi \left( p \right) = p - 1$ and $\phi \left( q \right) = q - 1$,  the previous result is equivalent to

\begin{align}
  a^{\phi \left( N \right)} = 1 \mod N &= a^{\phi \left( p \right) \, \phi \left( q \right)} \notag \\
  1 \mod N &= a^{\left(p - 1\right) \left(q - 1\right)} \notag
\end{align}






$a^{p - 1} = 1 \mod p$, and $a^{q - 1} = 1 \mod q$



























\end{flushleft}
\end{document}
